clean up and regularize journal chaining; before cleaning up journal API

Splinter/plan.i.dfy
@@ -107,35 +107,63 @@ module JournalMod {
   import opened Options
   import opened Sequences
   import opened Maps
+  import opened MsgSeqMod
   import opened MsgMapMod
   import opened AllocationMod
 
-  datatype Superblock = Superblock(firstCU: CU, firstValidSeq : nat)
+  datatype Superblock = Superblock(firstCU: Option<CU>, firstValidSeq : nat)
 
   // Monoid-friendly (quantified-list) definition
   datatype JournalRecord = JournalRecord(
-    messageMap: MsgMap,
+    messageSeq: MsgSeq,
     seqStart: nat,  // inclusive
-    seqEnd: nat,  // exclusive
     nextCU: Option<CU>   // linked list pointer
-  )
-  type JournalChain = seq<JournalRecord>
+  ) {
+
+    function seqEnd() : nat { seqStart + |messageSeq| }
+
+    // Synthesize a superblock that reflects the tail of the chain (cutting
+    // off the first rec), propagating along firstValidSeq.
+    function nextSB(sb: Superblock) : Superblock
+    {
+      Superblock(nextCU, sb.firstValidSeq)
+    }
+  }
+  datatype JournalChain = JournalChain(sb: Superblock, recs:seq<JournalRecord>)
+  {
+    // Synthesize a superblock that reflects the tail of the chain (cutting
+    // off the first rec), propagating along firstValidSeq.
+    function nextSB() : Superblock
+      requires 0<|recs|
+    {
+      recs[0].nextSB(sb)
+    }
+  }
 
   function parse(b: UninterpretedDiskPage) : Option<JournalRecord>
     // TODO marshalling
 
+  predicate IsLastLink(i: nat, chain: JournalChain)
+    requires 0<=i<|chain.recs|
+  {
+    // stop if nothing more available
+    || chain.recs[i].nextCU.None?
+    // stop if nothing more needed
+    || chain.sb.firstValidSeq >= chain.recs[i].seqStart
+  }
+
   predicate WFChainBasic(chain: JournalChain)
   {
-    && 0 < |chain|
-    && Last(chain).nextCU.None?
-    && (forall i | 0<=i<|chain|-1 :: chain[i].nextCU.Some?)
+    && (chain.sb.firstCU.None? <==> 0 == |chain.recs|)
+    && (forall i | 0<=i<|chain.recs| :: i==|chain.recs|-1 <==> IsLastLink(i, chain))
+    && (forall i | 0<=i<|chain.recs|-1 :: chain.recs[i].nextCU.Some?)
   }
 
   predicate {:opaque} WFChainInner(chain: JournalChain)
     requires WFChainBasic(chain)
   {
-    && (forall i | 0<=i<|chain|-1 ::
-      chain[i].seqStart == chain[i+1].seqEnd)
+    && (forall i | 0<=i<|chain.recs|-1 ::
+      chain.recs[i].seqStart == chain.recs[i+1].seqEnd())
   }
 
   predicate WFChain(chain: JournalChain)
@@ -144,12 +172,14 @@ module JournalMod {
     && WFChainInner(chain)
   }
 
-  function CUsForChain(firstCU: CU, chain: JournalChain) : (cus: seq<CU>)
+  function CUsForChain(chain: JournalChain) : (cus: seq<CU>)
     requires WFChain(chain)
-    ensures |cus| == |chain|
+    ensures |cus| == |chain.recs|
   {
-    [firstCU] + seq(|chain|-1,
-      i requires 0<=i<|chain|-1 => chain[i].nextCU.value)
+    if chain.sb.firstCU.None?
+    then []
+    else [chain.sb.firstCU.value] + seq(|chain.recs|-1,
+        i requires 0<=i<|chain.recs|-1 => chain.recs[i].nextCU.value)
   }
 
   predicate RecordOnDisk(dv: DiskView, cu: CU, journalRecord: JournalRecord)
@@ -158,86 +188,128 @@ module JournalMod {
     && parse(dv[cu]) == Some(journalRecord)
   }
 
-  predicate {:opaque} ChainMatchesDiskView(dv: DiskView, firstCU: CU, chain: JournalChain)
+  predicate {:opaque} ChainMatchesDiskView(dv: DiskView, chain: JournalChain)
     requires WFChain(chain)
   {
     // chain corresponds to stuff in the DiskView starting at firstCU.
-    && var cus := CUsForChain(firstCU, chain);
-    && (forall i | 0<=i<|chain| :: RecordOnDisk(dv, cus[i], chain[i]))
+    && var cus := CUsForChain(chain);
+    && (forall i | 0<=i<|chain.recs| :: RecordOnDisk(dv, cus[i], chain.recs[i]))
   }
 
   // Describe a valid chain with quantification.
-  predicate ValidJournalChain(dv: DiskView, firstCU: CU, chain: JournalChain)
+  predicate ValidJournalChain(dv: DiskView, chain: JournalChain)
   {
     && WFChain(chain)
-    && ChainMatchesDiskView(dv, firstCU, chain)
+    && ChainMatchesDiskView(dv, chain)
+  }
+
+  lemma ValidEmptyChain(dv: DiskView, sb: Superblock)
+    requires sb.firstCU.None?
+    ensures ValidJournalChain(dv, JournalChain(sb, []))
+  {
+    reveal_WFChainInner();
+    reveal_ChainMatchesDiskView();
+  }
+
+  function ExtendChain(sb: Superblock, rec: JournalRecord, innerchain: JournalChain)
+    : (chain: JournalChain)
+    requires sb.firstCU.Some?
+    requires rec.nextCU.Some? ==> sb.firstValidSeq < rec.seqStart; // proves !IsLastLink(0, chain)
+    requires innerchain.sb == rec.nextSB(sb);
+    requires 0<|innerchain.recs| ==> rec.seqStart == innerchain.recs[0].seqEnd();
+    requires WFChain(innerchain)
+    ensures WFChain(chain)
+  {
+    var chain := JournalChain(sb, [rec] + innerchain.recs);
+    assert WFChainBasic(chain) by {
+      forall i | 0<=i<|chain.recs| ensures i==|chain.recs|-1 <==> IsLastLink(i, chain)
+      {
+        if 0<i {
+          assert IsLastLink(i-1, innerchain) == IsLastLink(i, chain);
+        }
+      }
+    }
+    assert WFChainInner(chain) by { reveal_WFChainInner(); }
+    chain
   }
 
   // Define reading a chain recursively. Returns None if any of the
   // CUs point to missing blocks from the dv, or if the block can't
   // be parsed.
-  // Note that the firstCU.None? case is only here to clean up the recursive
-  // definition; that's why firstCU.Some? is a prereq for the ensures.
+  // Return the set of readCUs visited. We may read six CUs before returning
+  // a None chain. We have to know that to show how related dvs produce identical
+  // results (even when they're broken).
   datatype ChainResult = ChainResult(chain: Option<JournalChain>, readCUs:seq<CU>)
 
-  function ChainFromInner(dv: DiskView, firstCU: Option<CU>) : (r:ChainResult)
-    ensures firstCU.Some? && r.chain.Some?
-      ==> ValidJournalChain(dv, firstCU.value, r.chain.value)
+  function ChainFrom(dv: DiskView, sb: Superblock) : (r:ChainResult)
+    ensures r.chain.Some? ==>
+      && ValidJournalChain(dv, r.chain.value)
+      && r.chain.value.sb == sb
     decreases |dv.Keys|
   {
-    if firstCU.None? then
-      // Recursion stop condition. Didn't try to read anything
-      ChainResult(Some([]), [])
-    else if firstCU.value !in dv then
+    if sb.firstCU.None? then
+      // Superblock told the whole story; nothing to read.
+      ValidEmptyChain(dv, sb);
+      ChainResult(Some(JournalChain(sb, [])), [])
+    else if sb.firstCU.value !in dv then
       // !RecordOnDisk: tried to read firstCU and failed
-      ChainResult(None, [firstCU.value])
+      ChainResult(None, [sb.firstCU.value])
     else
-      var firstRec := parse(dv[firstCU.value]);
+      var firstRec := parse(dv[sb.firstCU.value]);
       if firstRec.None? then
         // !RecordOnDisk: read firstCU, but it was borked
-        ChainResult(None, [firstCU.value])
+        ChainResult(None, [sb.firstCU.value])
+      else if firstRec.value.seqEnd() <= sb.firstValidSeq then
+        // This isn't an invariant disk state: if we're in the initial call,
+        // the superblock shouldn't point to a useless JournalRecord; if we're
+        // in a recursive call with correctly-chained records, we should have
+        // already ignored this case.
+        ChainResult(None, [sb.firstCU.value])
+      else if firstRec.value.seqStart == sb.firstValidSeq then
+        // Glad we read this record, but we don't need to read anything beyond.
+        var r := ChainResult(Some(JournalChain(sb, [firstRec.value])), [sb.firstCU.value]);
+        assert ValidJournalChain(dv, r.chain.value) by {
+          reveal_WFChainInner();
+          reveal_ChainMatchesDiskView();
+        }
+        r
       else
-        var inner := ChainFromInner(MapRemove1(dv, firstCU.value), firstRec.value.nextCU);
+        var inner := ChainFrom(MapRemove1(dv, sb.firstCU.value), firstRec.value.nextSB(sb));
         if inner.chain.None? // tail didn't decode or
           // tail decoded but head doesn't stitch to it (a cross-crash invariant)
-          || (0<|inner.chain.value|
-              && firstRec.value.seqStart != inner.chain.value[0].seqEnd)
+          || (0<|inner.chain.value.recs|
+              && firstRec.value.seqStart != inner.chain.value.recs[0].seqEnd())
         then
           // failure in recursive call.
           // We read our cu plus however far the recursive call reached.
-          ChainResult(None, [firstCU.value] + inner.readCUs)
+          ChainResult(None, [sb.firstCU.value] + inner.readCUs)
         else
-          var chain := [firstRec.value] + inner.chain.value;
-          assert ValidJournalChain(dv, firstCU.value, chain) by {
-            reveal_WFChainInner();
+          assert firstRec.value.nextCU.Some? ==> sb.firstValidSeq < firstRec.value.seqStart;
+          var chain := ExtendChain(sb, firstRec.value, inner.chain.value);
+          //var chain := JournalChain(sb, [firstRec.value] + inner.chain.value.recs);
+          assert ValidJournalChain(dv, chain) by {
             reveal_ChainMatchesDiskView();
-            var cus := CUsForChain(firstCU.value, chain);
-            assert forall i | 0<=i<|chain| :: RecordOnDisk(dv, cus[i], chain[i]); // trigger
+            var cus := CUsForChain(chain);
+            assert forall i | 0<=i<|chain.recs| :: RecordOnDisk(dv, cus[i], chain.recs[i]); // trigger
           }
-          ChainResult(Some(chain), [firstCU.value] + inner.readCUs)
+          ChainResult(Some(chain), [sb.firstCU.value] + inner.readCUs)
   }
 
-  // Returns None if any of the CUs point to missing blocks from the dv, or if
-  // the block can't be parsed.
-  function ChainFrom(dv: DiskView, firstCU: CU) : (chain:Option<JournalChain>)
+  // TODO redo: return a seq of Message, with a prefix of None.
+  function MessageMaps(journalChain: JournalChain) : seq<MsgSeq> {
+    seq(|journalChain.recs|,
+      i requires 0<=i<|journalChain.recs|
+        => var mm := journalChain.recs[i].messageSeq; mm)
+  }
+
+  function IM(dv: DiskView, sb: Superblock) : seq<MsgSeq>
   {
-    ChainFromInner(dv, Some(firstCU)).chain
-  }
-
-  function MessageMaps(journalChain: JournalChain) : seq<MsgMap> {
-    seq(|journalChain|,
-      i requires 0<=i<|journalChain|
-        => var mm := journalChain[i].messageMap; mm)
-  }
-
-  function IM(dv: DiskView, sb: Superblock) : MsgMap
-  {
-    var chain := ChainFrom(dv, sb.firstCU);
+    var chain := ChainFrom(dv, sb).chain;
     if chain.Some?
     then
-      MsgMapMod.ConcatSeq(MessageMaps(chain.value))
+      MessageMaps(chain.value)
     else
-      MsgMapMod.Empty()
+      []
   }
 
   function ReadAt(cus: seq<CU>, i: nat) : AU
@@ -246,9 +318,9 @@ module JournalMod {
     cus[i].au
   }
 
-  function IReads(dv: DiskView, firstCU: CU) : seq<AU>
+  function IReads(dv: DiskView, sb: Superblock) : seq<AU>
   {
-    var cus := ChainFromInner(dv, Some(firstCU)).readCUs;
+    var cus := ChainFrom(dv, sb).readCUs;
     // wanted to write:
     // seq(|cus|, i requires 0<=i<|cus| => cus[i].au)
     // but Dafny bug, so:
@@ -266,37 +338,6 @@ module JournalMod {
     forall cu:CU :: cu.au in aus ==> EqualAt(dv0, dv1, cu)
   }
 
-  lemma ValidTruncatedChain(dv: DiskView, firstCU: CU, c: JournalChain)
-    requires ValidJournalChain(dv, firstCU, c)
-    requires 1<|c|
-    ensures c[0].nextCU.Some? // boilerplate for next line
-    ensures ValidJournalChain(dv, c[0].nextCU.value, c[1..])
-  {
-    reveal_ChainMatchesDiskView();
-    reveal_WFChainInner();
-  }
-
-  lemma UniqueChain(dv: DiskView, firstCU: CU, c0: JournalChain, c1: JournalChain)
-    requires ValidJournalChain(dv, firstCU, c0)
-    requires ValidJournalChain(dv, firstCU, c1)
-    ensures c0 == c1
-    decreases |c0|
-  {
-    reveal_ChainMatchesDiskView();
-    if |c1|<|c0| {
-      UniqueChain(dv, firstCU, c1, c0);
-    } else {
-      assert c0[0]==c1[0];
-      if 1==|c0| {
-        assert 1==|c1|;
-      } else {
-        ValidTruncatedChain(dv, firstCU, c0);
-        ValidTruncatedChain(dv, firstCU, c1);
-        UniqueChain(dv, c0[0].nextCU.value, c0[1..], c1[1..]);
-      }
-    }
-  }
-
   predicate SequenceSubset<T>(a:seq<T>, b:seq<T>)
   {
     forall i | 0<=i<|a| :: a[i] in b
@@ -309,41 +350,50 @@ module JournalMod {
   {
   }
 
-  lemma FrameOneChain(dv0: DiskView, dv1: DiskView, firstCU: Option<CU>, chain: Option<JournalChain>)
-    requires chain == ChainFromInner(dv0, firstCU).chain
-    requires firstCU.Some? ==> DiskViewsEquivalentForSet(dv0, dv1, IReads(dv0, firstCU.value))
-    ensures chain == ChainFromInner(dv1, firstCU).chain
+  lemma FrameOneChain(dv0: DiskView, dv1: DiskView, sb: Superblock, chain: Option<JournalChain>)
+    requires chain == ChainFrom(dv0, sb).chain
+    requires DiskViewsEquivalentForSet(dv0, dv1, IReads(dv0, sb))
+    ensures chain == ChainFrom(dv1, sb).chain
   {
-    if firstCU.Some? {
-      assert IReads(dv0, firstCU.value)[0] == firstCU.value.au; // trigger
-      if firstCU.value in dv0 {
-        var firstRec := parse(dv0[firstCU.value]);
+    if sb.firstCU.Some? {
+      assert IReads(dv0, sb)[0] == sb.firstCU.value.au; // trigger
+      if sb.firstCU.value in dv0 {
+        var firstRec := parse(dv0[sb.firstCU.value]);
         if firstRec.Some? { // Recurse to follow chain
-          var dv0r := MapRemove1(dv0, firstCU.value);
-          var nextCU := firstRec.value.nextCU;
-          var aus := IReads(dv0, firstCU.value);
-          var ausr := if nextCU.Some? then IReads(dv0r, nextCU.value) else [];
+          if firstRec.value.seqEnd() <= sb.firstValidSeq {
+          } else if firstRec.value.seqStart == sb.firstValidSeq {
+          } else {
+            var dv0r := MapRemove1(dv0, sb.firstCU.value);
+            var nextCU := firstRec.value.nextCU;
+            var nextSB := firstRec.value.nextSB(sb);
+            var aus := IReads(dv0, sb);
+            var ausr := if nextCU.Some?
+              then IReads(dv0r, nextSB)
+              else [];
 
-          forall i | 0<=i<|ausr| ensures ausr[i] in aus {
-            assert aus[i+1] == ausr[i]; // witness to SequenceSubset(ausr, aus)
+            forall i | 0<=i<|ausr| ensures ausr[i] in aus {
+              assert aus[i+1] == ausr[i]; // witness to SequenceSubset(ausr, aus)
+            }
+            DiskViewsEquivalentAfterRemove(dv0, dv1, aus, sb.firstCU.value, ausr);
+            FrameOneChain(dv0r, MapRemove1(dv1, sb.firstCU.value),
+              nextSB, ChainFrom(dv0r, nextSB).chain);
           }
-          DiskViewsEquivalentAfterRemove(dv0, dv1, aus, firstCU.value, ausr);
-          FrameOneChain(dv0r, MapRemove1(dv1, firstCU.value),
-            nextCU, ChainFromInner(dv0r, nextCU).chain);
         }
       }
     }
   }
 
   lemma Framing(sb:Superblock, dv0: DiskView, dv1: DiskView)
-    requires DiskViewsEquivalentForSet(dv0, dv1, IReads(dv0, sb.firstCU))
+    requires DiskViewsEquivalentForSet(dv0, dv1, IReads(dv0, sb))
     ensures IM(dv0, sb) == IM(dv1, sb)
   {
-    FrameOneChain(dv0, dv1, Some(sb.firstCU), ChainFrom(dv0, sb.firstCU));
+    FrameOneChain(dv0, dv1, sb, ChainFrom(dv0, sb).chain);
   }
 }
 
 module MarshalledSnapshot {
+  // A snapshot of a data structure, spread across a linked list of CUs on the disk.
+  // This module almost certainly shares a bunch of DNA with Journal; TODO refactor.
   import opened AllocationMod
   import opened NativeTypes
 
@@ -536,7 +586,9 @@ module System {
     var sb := ISuperblock(dv);
     if sb.Some?
     then
-      JournalMod.IM(dv, sb.value.journal) + BetreeMod.IM(dv, sb.value.betree)
+      //JournalMod.IM(dv, sb.value.journal) + BetreeMod.IM(dv, sb.value.betree)
+      // TODO stubbed out because IM API is changing to MsgSeqs
+      BetreeMod.IM(dv, sb.value.betree)
     else
       MsgMapMod.Empty()
   }
